cfrontend/BeePL_typesystem.v
@@ -10,70 +10,68 @@ Definition type_bool (t : type) : Prop :=
 classify_bool t <> bool_default. 
 
 Inductive type_expr : ty_context -> store_context -> expr -> effect -> type -> Prop :=
-| Ty_val_unit : forall Gamma Sigma,
-                type_expr Gamma Sigma (Val Vunit (Ptype Tunit)) empty_effect (Ptype Tunit)
-| Ty_val_int : forall Gamma Sigma i sz s a,
-               type_expr Gamma Sigma (Val (Vint i) (Ptype (Tint sz s a))) empty_effect (Ptype (Tint sz s a))
-| Ty_val_long : forall Gamma Sigma i s a,
-               type_expr Gamma Sigma (Val (Vint64 i) (Ptype (Tlong s a))) empty_effect (Ptype (Tlong s a))
-| Ty_val_loc : forall Gamma Sigma h t l ofs a,
-               type_expr Gamma Sigma (Val (Vloc l ofs) (Reftype h (Bprim t) a)) empty_effect (Reftype h (Bprim t) a) 
-| Ty_var : forall Gamma Sigma x t, 
+| ty_val : forall Gamma Sigma v t,
+           type_expr Gamma Sigma (Val v t) empty_effect t
+| ty_var : forall Gamma Sigma x t, 
            PTree.get x.(vname) (extend_context Gamma x.(vname) t) = Some t ->
            x.(vtype) = t ->
            type_expr Gamma Sigma (Var x) empty_effect t
-| Ty_constint : forall Gamma Sigma t sz s a i,
+| ty_constint : forall Gamma Sigma t sz s a i,
                 t = (Ptype (Tint sz s a)) ->
                 type_expr Gamma Sigma (Const (ConsInt i) t) empty_effect t
-| Ty_constlong : forall Gamma Sigma t s a i,
+| ty_constlong : forall Gamma Sigma t s a i,
                  t = (Ptype (Tlong s a)) ->
                  type_expr Gamma Sigma (Const (ConsLong i) t) empty_effect t
-| Ty_constunit : forall Gamma Sigma t,
+| ty_constunit : forall Gamma Sigma t,
                  t = (Ptype Tunit) ->
                  type_expr Gamma Sigma (Const (ConsUnit) t) empty_effect t
 (* Fix me *)
-| Ty_app : forall Gamma Sigma e es rt efs ts ef efs', 
+| ty_app : forall Gamma Sigma e es rt efs ts ef efs', 
            type_expr Gamma Sigma e ef (Ftype ts efs rt) -> 
            type_exprs Gamma Sigma es efs' ts -> 
            type_expr Gamma Sigma (App e es rt) (ef ++ efs ++ efs') rt
-| Ty_prim_ref : forall Gamma Sigma e ef h bt a, 
+| ty_prim_ref : forall Gamma Sigma e ef h bt a, 
                 type_expr Gamma Sigma e ef (Ptype bt) ->
                 type_expr Gamma Sigma (Prim Ref (e::nil) (Reftype h (Bprim bt) a)) (ef ++ (Alloc h :: nil)) (Reftype h (Bprim bt) a) 
-| Ty_prim_deref : forall Gamma Sigma e ef h bt a, (* inner expression should be unrestricted as it will be used later *)
+| ty_prim_deref : forall Gamma Sigma e ef h bt a, (* inner expression should be unrestricted as it will be used later *)
                   type_expr Gamma Sigma e ef (Reftype h (Bprim bt) a) -> 
                   type_expr Gamma Sigma (Prim Deref (e::nil) (Ptype bt)) (ef ++ (Read h :: nil)) (Ptype bt)
-| Ty_prim_massgn : forall Gamma Sigma e e' h bt ef a ef', 
+| ty_prim_massgn : forall Gamma Sigma e e' h bt ef a ef', 
                    type_expr Gamma Sigma e ef (Reftype h (Bprim bt) a) ->
                    type_expr Gamma Sigma e' ef' (Ptype bt) ->
                    type_expr Gamma Sigma (Prim Massgn (e::e'::nil) (Ptype Tunit)) (ef ++ ef' ++ (Write h :: nil)) (Ptype Tunit)
-| Ty_prim_uop : forall Gamma Sigma op e ef t,
+| ty_prim_uop : forall Gamma Sigma op e ef t,
                 type_expr Gamma Sigma e ef t ->
                 type_expr Gamma Sigma (Prim (Uop op) (e::nil) t) ef t
-| Ty_prim_bop : forall Gamma Sigma op e ef t e',
+| ty_prim_bop : forall Gamma Sigma op e ef t e',
                 type_expr Gamma Sigma e ef t ->
                 type_expr Gamma Sigma e' ef t ->
                 type_expr Gamma Sigma (Prim (Bop op) (e::e'::nil) t) ef t 
-| Ty_bind : forall Gamma Sigma x t e e' t' ef ef',
+| ty_bind : forall Gamma Sigma x t e e' t' ef ef',
             type_expr Gamma Sigma e ef t ->
             type_expr (extend_context Gamma x t) Sigma e' ef' t' ->
             type_expr Gamma Sigma (Bind x t e e' t') (ef ++ ef') t'
-| Ty_cond : forall Gamma Sigma e1 e2 e3 tb t ef1 ef2 ef3, 
+| ty_cond : forall Gamma Sigma e1 e2 e3 tb t ef1 ef2 ef3, 
             type_expr Gamma Sigma e1 ef1 tb ->
             type_bool tb ->
             type_expr Gamma Sigma e2 ef2 t ->
             type_expr Gamma Sigma e3 ef3 t ->
             type_expr Gamma Sigma (Cond e1 e2 e3 t) (ef1 ++ ef2 ++ ef3) t
-| Ty_unit : forall Gamma Sigma,
+| ty_unit : forall Gamma Sigma,
             type_expr Gamma Sigma (Unit (Ptype Tunit)) empty_effect (Ptype Tunit)
-| Ty_addr : forall Gamma Sigma l ofs h t a,
+| ty_addr : forall Gamma Sigma l ofs h t a,
             l.(ltype) = Reftype h (Bprim t) a ->
             type_expr Gamma Sigma (Addr l ofs) empty_effect l.(ltype) 
-(* fix me : Run, Hexpr *)
+(* fix me : Run *)
+(* fix me : Hexpr *)
+(*| ty_hexpr : forall Gamma Sigma m e h ef t a, 
+             type_expr Gamma Sigma e ef (Reftype h (Bprim t) a) ->
+             type_expr Gamma Sigma (Hexpr m e (Reftype h (Bprim t) a)) ef (Reftype h (Bprim t) a)*)
 (* fix me : Add typing rule for external function *)
 with type_exprs : ty_context -> store_context -> list expr -> effect -> list type -> Prop :=
-| Ty_nil : forall Gamma Sigma,
+| ty_nil : forall Gamma Sigma,
            type_exprs Gamma Sigma nil nil nil
-| Ty_cons : forall Gamma Sigma e es ef efs t ts,
+| ty_cons : forall Gamma Sigma e es ef efs t ts,
             type_expr Gamma Sigma e ef t ->
             type_exprs Gamma Sigma es efs ts ->
             type_exprs Gamma Sigma (e :: es) (ef ++ efs) (t :: ts).
@@ -82,17 +80,27 @@ Scheme type_expr_ind_mut := Induction for type_expr Sort Prop
   with type_exprs_ind_mut := Induction for type_exprs Sort Prop.
 Combined Scheme type_exprs_type_expr_ind_mut from type_exprs_ind_mut, type_expr_ind_mut.
 
+(* The (EXTEND) rule states that we can always assume a worse effect; 
+   this rule is not part of the inference rules but
+   we need it to show subject reduction of stateful computations. : Leijen's koka paper *)
+(* This hypothesis makes the type system non-deterministic *)
+Hypothesis ty_extend : forall Gamma Sigma e t ef, 
+                        type_expr Gamma Sigma e empty_effect t ->
+                        type_expr Gamma Sigma e (ef ++ empty_effect) t.
+
 Section type_expr_ind.
 Context (Pts : ty_context -> store_context -> list expr -> effect -> list type -> Prop).
 Context (Pt : ty_context -> store_context -> expr -> effect -> type -> Prop).
-Context (Htvalu : forall Gamma Sigma,
+Context (Htval : forall Gamma Sigma v t,
+                 Pt Gamma Sigma (Val v t) empty_effect t).
+(*Context (Htvalu : forall Gamma Sigma,
                   Pt Gamma Sigma (Val Vunit (Ptype Tunit)) empty_effect (Ptype Tunit)).
 Context (Htvali Ty_val_int : forall Gamma Sigma i sz s a,
                              Pt Gamma Sigma (Val (Vint i) (Ptype (Tint sz s a))) empty_effect (Ptype (Tint sz s a))).
 Context (Htvall : forall Gamma Sigma i s a,
                   Pt Gamma Sigma (Val (Vint64 i) (Ptype (Tlong s a))) empty_effect (Ptype (Tlong s a))).
 Context (Htvalloc : forall Gamma Sigma h t l ofs a,
-                    Pt Gamma Sigma (Val (Vloc l ofs) (Reftype h (Bprim t) a)) empty_effect (Reftype h (Bprim t) a)). 
+                    Pt Gamma Sigma (Val (Vloc l ofs) (Reftype h (Bprim t) a)) empty_effect (Reftype h (Bprim t) a)). *)
 Context (Htvar : forall Gamma Sigma x t,
                  PTree.get x.(vname) (extend_context Gamma x.(vname) t) = Some t ->
                  x.(vtype) = t ->
@@ -142,6 +150,9 @@ Context (Htunit : forall Gamma Sigma,
 Context (Htloc : forall Gamma Sigma l h bt a ofs, 
                  l.(ltype) = (Reftype h bt a) ->
                  Pt Gamma Sigma (Addr l ofs) empty_effect l.(ltype)). 
+(*Context (Htheap : forall Gamma Sigma m e h ef t a, 
+                  Pt Gamma Sigma e ef (Reftype h (Bprim t) a) ->
+                  Pt Gamma Sigma (Hexpr m e (Reftype h (Bprim t) a)) ef (Reftype h (Bprim t) a)).*)
 Context (Htnil : forall Gamma Sigma,
                  Pts Gamma Sigma nil nil nil).
 Context (Htcons : forall Gamma Sigma e es t ef ts efs,
@@ -184,6 +195,8 @@ apply type_exprs_type_expr_ind_mut=> //=.
   by apply Htcond with tb.
 (* Addr *)
 + move=> Gamma Sigma l ofs h t a hteq; subst. by apply Htloc with h (Bprim t) a.
+(* Hexpr 
++ move=> Gamma Sigma m e h ef t a hte ht. by apply Htheap.*)
 move=> Gamma Sigma e es ef efs t ts hte ht htes hts.
 by apply Htcons.
 Qed.
@@ -210,10 +223,7 @@ suff : (forall Gamma Sigma es efs ts, type_exprs Gamma Sigma es efs ts ->
   move=> Gamma Sigma e ef t ef' t' he he'.
   by move: (ih' Gamma Sigma e ef t he ef' t' he').
 apply type_expr_indP => //=.
-+ by move=> Gamma Sigma ef' t' ht; inversion ht; subst.
-+ by move=> Gamma Sigma i sz s a ef' t' ht; inversion ht; subst.
-+ by move=> Gamma Sigma i s a ef' t' ht; inversion ht; subst.
-+ by move=> Gamma Sigma h t l ofs a ef' t' ht; inversion ht; subst.
++ by move=> Gamma Sigma v t ef' t' ht; inversion ht; subst.
 + move=> Gamma Sigma x t htx ht ef' t' het; subst. by inversion het; subst.
 + move=> Gamma Sigma t sz s i a ht ef' t' ht'; subst. by inversion ht'; subst.
 + move=> Gamma Sigma t s i a ht ef' t' ht'; subst. by inversion ht'; subst.
@@ -254,8 +264,8 @@ Qed.
 
 Lemma eq_type_rel : forall v t t',
 eq_type t t' ->
-typeof_value v (wtype_of_type t') ->
-typeof_value v (wtype_of_type t).
+wtypeof_value v (wtype_of_type t') ->
+wtypeof_value v (wtype_of_type t).
 Proof.
 move=> v t t'. case: t=> //=.
 + move=> p. case: t'=> //= p'.
@@ -277,9 +287,17 @@ Qed.
    the assumption we made about [x] when typing [e], we should be
    able to substitute [e'] for each of the occurrences of [x] in [e]
    and obtain a new expression that still has type [t]. *)
+Lemma wsubst_preservation : forall Gamma Sigma bge vm hm hm' x t v e ef t' e'', 
+type_expr (extend_context Gamma x.(vname) t) Sigma e ef t' ->
+wtypeof_value v (wtype_of_type t) ->
+subst bge vm hm x.(vname) v e hm' e'' ->
+type_expr Gamma Sigma e'' ef t'.
+Proof.
+Admitted.
+
 Lemma subst_preservation : forall Gamma Sigma bge vm hm hm' x t v e ef t' e'', 
 type_expr (extend_context Gamma x.(vname) t) Sigma e ef t' ->
-typeof_value v (wtype_of_type t) ->
+typeof_value v t ->
 subst bge vm hm x.(vname) v e hm' e'' ->
 type_expr Gamma Sigma e'' ef t'.
 Proof.
@@ -342,9 +360,9 @@ case: ty=> //=.
 move=> f. by case: f=> //=.
 Qed.
 
-Lemma bty_chunk_rel : forall (ty: type) chunk,
+Lemma wbty_chunk_rel : forall (ty: type) chunk,
 access_mode ty = By_value (transl_bchunk_cchunk chunk) ->
-(wtype_of_type ty) = (typeof_chunk chunk).
+(wtype_of_type ty) = (wtypeof_chunk chunk).
 Proof.  
 move=> ty chunk. case: chunk=> //=; case: ty=> //= p; case: p=> //=.
 move=> i s a. case: i=> //=.
@@ -352,20 +370,10 @@ move=> i s a. case: i=> //=.
 case: s=> //=.
 Qed.
 
-(*Lemma bty_chunk_rel' : forall (ty: type) chunk,
-access_mode ty = By_value (transl_memory_chunk chunk) ->
-ty = (typeof_chunk chunk).
-Proof.  
-move=> ty chunk. case: chunk=> //=; case: ty=> //= p; case: p=> //=.
-move=> i s a. case: i=> //=.
-+ by case: s=> //=.
-case: s=> //=.
-Qed.*)
-
 Lemma cval_bval_type_chunk : forall v chunk v',
 Values.Val.has_type v (type_of_chunk (transl_bchunk_cchunk chunk)) ->
 transC_val_bplvalue v = Errors.OK v' ->
-typeof_value v' (typeof_chunk chunk). 
+wtypeof_value v' (wtypeof_chunk chunk). 
 Proof.
 move=> v chunk v'. by case: chunk=> //=; case: v=> //=; case: v'=> //=. 
 Qed.
@@ -375,42 +383,26 @@ Lemma cval_bval_type_eq : forall v ct v' bt g g' i,
 Values.Val.has_type v (typ_of_type ct) ->
 transC_val_bplvalue v = Errors.OK v' ->
 transBeePL_type bt g = SimplExpr.Res ct g' i ->
-typeof_value v' (wtype_of_type bt). 
+wtypeof_value v' (wtype_of_type bt). 
 Proof.
 Admitted.
  
 (* Complete me *) (* Medium level *)
-Lemma deref_addr_val_ty : forall bge ty m l ofs bf v,
+Lemma wderef_addr_val_ty : forall bge ty m l ofs bf v,
 deref_addr bge ty m l ofs bf v ->
-typeof_value v (wtype_of_type ty).
+wtypeof_value v (wtype_of_type ty).
 Proof.
 move=> bge ty m l ofs bf v hd. inversion hd; subst.
 + rewrite /Mem.loadv /= in H2.
   have hvt := Mem.load_type m (transl_bchunk_cchunk chunk) l 
               (Ptrofs.unsigned ofs) v0 H1.
-  have hwt := bty_chunk_rel ty chunk H.
-  rewrite /typeof_value /= hwt /typeof_chunk /=. 
+  have hwt := wbty_chunk_rel ty chunk H.
+  rewrite /wtypeof_value /= hwt /wtypeof_chunk /=. 
   by case: chunk H H1 hvt hwt=> //=; case: v hd H2=> //=; case: v0=> //=.
 + admit. (* complete me for the case of volatile load *)
 case: ty hd H=> //= p. case: p=> //= i s a.
 by case: i=> //=;case: s=> //=.
 Admitted.
-
-(* Value typing *)
-(* A value does not produce any effect *)
-Lemma value_typing : forall Gamma Sigma ef t v,
-type_expr Gamma Sigma (Val v t) ef t ->
-ef = empty_effect.
-Proof.
-move=> Gamma Sigma ef t v ht. elim: v ht=> //=.
-(* unit *)
-+ move=> ht. by inversion ht.
-(* int *)
-+ move=> i ht. by inversion ht.
-(* long *)
-+ move=> i ht. by inversion ht.
-move=> l ofs ht. by inversion ht.
-Qed.
 
 (* Complete Me *)
 Lemma uop_type_preserve : forall uop v ct m v',
@@ -424,7 +416,7 @@ transBeePL_type t g = SimplExpr.Res ct g' i ->
 Cop.sem_unary_operation uop v ct m = Some v' ->
 Values.Val.has_type v' (typ_of_type ct) ->
 transC_val_bplvalue v' = Errors.OK v'' -> 
-typeof_value v'' (wtype_of_type t).
+wtypeof_value v'' (wtype_of_type t).
 Proof.
 Admitted.
 
@@ -443,44 +435,180 @@ Cop.sem_binary_operation cenv op v1 ct1 v2 ct2 m = Some v ->
 transC_val_bplvalue v = Errors.OK v' ->
 Values.Val.has_type v (typ_of_type ct1) ->
 Values.Val.has_type v (typ_of_type ct2) ->
-typeof_value v' (wtype_of_type t1) /\ typeof_value v' (wtype_of_type t2).
+wtypeof_value v' (wtype_of_type t1) /\ wtypeof_value v' (wtype_of_type t2).
 Proof.
 Admitted.
 
+Lemma type_to_wtype : forall v t,
+typeof_value v t ->
+wtypeof_value v (wtype_of_type t).
+Proof.
+move=> v t. case: t=> //=.
++ move=> p. case: p=> //=.
+  + move=> i s a. by case: v=> //=.
+  move=> s a. by case: v=> //=.
++ move=> h b a. by case: v=> //=.
+move=> es e t. by case: v=> //=.
+Qed.
+
+(* Value typing *)
+(* A value does not produce any effect *)
+Lemma value_typing : forall Gamma Sigma ef t v,
+type_expr Gamma Sigma (Val v t) ef t ->
+ef = empty_effect.
+Proof.
+move=> Gamma Sigma ef t v ht. elim: v ht=> //=.
+(* unit *)
++ move=> ht. by inversion ht.
+(* int *)
++ move=> i ht. by inversion ht.
+(* long *)
++ move=> i ht. by inversion ht.
+move=> l ofs ht. by inversion ht.
+Qed.
+
+(*** Proving theorems related to type system for small step semantics of BeePL *)
+Lemma progress_ssem_expr_exprs:
+(forall Gamma Sigma es efs ts bge vm m, type_exprs Gamma Sigma es efs ts ->
+                                        is_values es \/ exists m' vm' es',
+                                                        ssem_exprs bge vm m es m' vm' es') /\
+(forall Gamma Sigma e ef t bge vm m, type_expr Gamma Sigma e ef t ->
+                                               is_value e \/ exists m' vm' e', 
+                                                             ssem_expr bge vm m e m' vm' e').
+Proof.
+Admitted.
+
+
+Lemma subject_reduction_ssem_expr_exprs: 
+(forall Gamma Sigma es efs ts bge vm m vm' m' es', type_exprs Gamma Sigma es efs ts ->
+                                                   ssem_exprs bge vm m es m' vm' es' ->
+                                                   type_exprs Gamma Sigma es' efs ts) /\
+(forall Gamma Sigma e ef t bge vm m vm' m' e', type_expr Gamma Sigma e ef t ->
+                                               ssem_expr bge vm m e m' vm' e' ->
+                                               type_expr Gamma Sigma e' ef t).
+Proof.
+suff : (forall Gamma Sigma es efs ts, type_exprs Gamma Sigma es efs ts ->
+                                      forall bge vm m vm' m' es', ssem_exprs bge vm m es m' vm' es' ->
+                                                                  type_exprs Gamma Sigma es' efs ts) /\
+       (forall Gamma Sigma e ef t, type_expr Gamma Sigma e ef t ->
+                                   forall bge vm m vm' m' e', ssem_expr bge vm m e m' vm' e' ->
+                                                             type_expr Gamma Sigma e' ef t).
+Proof.
++ move=> [] ih ih'. split=> //=.
+  + move=> Gamma Sigma es efs ts bge vm m vm' m' es' hts hes.
+    by move: (ih Gamma Sigma es efs ts hts bge vm m vm' m' es' hes).
+  move=> Gamma Sigma e ef t bge vm m vm' m' e' ht he.
+  by move: (ih' Gamma Sigma e ef t ht bge vm m vm' m' e' he).
+apply type_expr_indP=> //=.
+(* val *)
++ move=> Gamma Sigma v t bge vm m vm' m' e' he.
+  inversion he; subst. by apply ty_val.
+(* var *)
++ move=> Gamma Sigma x t ht hteq bge vm m vm' m' e' he.
+  by inversion he; subst; apply ty_val. 
+(* const int *)
++ move=> Gamma Sigma t sz s i a hteq bge vm m vm' m' e' he.
+  inversion he; subst. by apply ty_val.
+(* const long *)
++ move=> Gamma Sigma t s i a hteq bge vm m vm' m' e' he.
+  inversion he; subst. by apply ty_val.
+(* const unit *)
++ move=> Gamma Sigma t hteq bge vm m vm' m' e' he.
+  inversion he; subst. by apply ty_val.
+(* app *)
++ move=> Gamma Sigma e es rt ef efs ts efs' hie hies bge vm m vm' m' e' he.
+  inversion he; subst.
+  (* fd location e and es takes step *) 
+  + apply ty_app with ts.   
+    + by move: (hie bge vm m vm' m' e'0 H7). admit.
+  (* takes step to body of function *)
+  admit.
+(* ref *)
++ move=> Gamma Sigma e ef h bt a hie bge vm m vm' m' e' he.
+  inversion he; subst.
+  + apply ty_prim_ref. by move: (hie bge vm m vm' m' e'0 H8).
+  have heq : (ef ++ [:: Alloc h]) = (ef ++ [:: Alloc h] ++ empty_effect).
+  + rewrite /empty_effect. by rewrite cats0. rewrite heq.
+  have hl : type_expr Gamma Sigma (Val (Vloc l ofs) (Reftype h (Bprim bt) a)) empty_effect
+     (Reftype h (Bprim bt) a). + by apply ty_val.
+  have het := ty_extend Gamma Sigma (Val (Vloc l ofs) (Reftype h (Bprim bt) a)) 
+          (Reftype h (Bprim bt) a) (ef ++ [:: Alloc h]) hl. by rewrite catA.
+(* deref *)
++ move=> Gamma Sigma e ef h bt a hie bge vm m vm' m' e' he.
+  inversion he; subst.
+  (* e takes step *)
+  + apply ty_prim_deref with a. by move: (hie bge vm m vm' m' e'0 H6).
+  (* e is a value *)
+  have heq : (ef ++ [:: Read h]) = (ef ++ [:: Read h] ++ empty_effect).
+  + rewrite /empty_effect. by rewrite cats0. rewrite heq.
+  have hl : type_expr Gamma Sigma (Val v (Ptype bt)) empty_effect
+     (Ptype bt). + by apply ty_val.
+  have het := ty_extend Gamma Sigma (Val v (Ptype bt))
+              (Ptype bt) (ef ++ [:: Read h]) hl. by rewrite catA.
+(* massgn *)
++ move=> Gamma Sigma e1 e2 ef1 ef2 h bt a hie1 hie2 bge vm m vm' m' e' he.
+  inversion he; subst.
+  (* e1 takes step *)
+  + apply ty_prim_massgn with bt a.
+    + by move: (hie1 bge vm m vm' m' e1' H6).
+    admit. (* why we don't have hypothesis for type of e2 *)
+  (* e2 takes step *)
+  + apply ty_prim_massgn with bt a0. admit.
+    by move : (hie2 bge vm m vm' m' e2' H6)=> ht2.
+  have hvt : type_expr Gamma Sigma (Val Vunit (Ptype Tunit))
+  empty_effect (Ptype Tunit). + by apply ty_val.
+  have het := ty_extend Gamma Sigma (Val Vunit (Ptype Tunit)) (Ptype Tunit) ((ef1 ++ ef2) ++ [:: Write h]) hvt.
+  rewrite /empty_effect cats0 in het. by rewrite catA.
+(* uop *)
++ move=> Gamma Sigma op e ef t hie bge vm m vm' m' e' he. inversion he; subst.
+  + apply ty_prim_uop. by move: (hie bge vm m vm' m' e'0 H7).
+    have hvt : type_expr Gamma Sigma (Val v'' t) empty_effect t. + by apply ty_val.
+    have := ty_extend Gamma Sigma (Val v'' t) t ef.
+Admitted.
+  
+  
+(*** Proving theorems related to type system for big step semantics of BeePL *)
 Lemma subject_reduction_bsem_expr_exprs: 
 (forall Gamma Sigma es efs ts bge vm m vm' m' vs, type_exprs Gamma Sigma es efs ts ->
                                                   bsem_exprs bge vm m es m' vm' vs ->
-                                                  typeof_values vs (wtypes_of_types ts)) /\
+                                                  wtypeof_values vs (wtypes_of_types ts)) /\
 (forall Gamma Sigma e ef t bge vm m vm' m' v, type_expr Gamma Sigma e ef t ->
                                               bsem_expr bge vm m e m' vm' v ->
-                                              typeof_value v (wtype_of_type t)).
+                                              wtypeof_value v (wtype_of_type t)).
 Proof.
 suff : (forall Gamma Sigma es efs ts, type_exprs Gamma Sigma es efs ts ->
                                       forall bge vm m vm' m' vs, bsem_exprs bge vm m es m' vm' vs ->
-                                                                 typeof_values vs (wtypes_of_types ts)) /\
+                                                                 wtypeof_values vs (wtypes_of_types ts)) /\
        (forall Gamma Sigma e ef t, type_expr Gamma Sigma e ef t ->
                                    forall bge vm m vm' m' v, bsem_expr bge vm m e m' vm' v ->
-                                                             typeof_value v (wtype_of_type t)).
+                                                             wtypeof_value v (wtype_of_type t)).
 + move=> [] ih ih'. split=> //=.
   + move=> Gamma Sigma es efs ts bge vm m m' vm' vs hts hes. 
     by move: (ih Gamma Sigma es efs ts hts bge vm m m' vm' vs hes).
   move=> Gamma Sigma e ef t bge vm m m' vm' v ht he.
   by move: (ih' Gamma Sigma e ef t ht bge vm m m' vm' v he).
 apply type_expr_indP => //=.
-(* val unit *)
-+ move=> Gamma Sigma bge vm m vm' m' v hv. by inversion hv; subst.
-(* val int *)
-+ move=> Gamma Sigma i sz s a bge vm m vm' m' v hv. by inversion hv; subst.
-(* val long *)
-+ move=> Gamma Sigma i s a bge vm m vm' m' v hv. by inversion hv; subst.
-(* val loc *)
-+ move=> Gamma Sigma h t l ofs a bge vm m vm' m' v hv. by inversion hv; subst.
+(* val *)
++ move=> Gamma Sigma v t bge vm m vm' m' v' he. inversion he; subst.
+  case: t he H6=> //=.
+  + move=> p. case: p=> //=.
+    + move=> he hw. case: v' he hw=> //=.
+      + move=> i he hw. by inversion hw.
+      + move=> i he hw. by inversion hw.
+      move=> l ofs he hw. by inversion hw.
+    + move=> i s a he hw. case: v' he hw=> //=.
+      + move=> i' he hw. by inversion hw.
+      move=> l ofs he hw. by inversion hw.
+    + move=> s a he hw. case: v' he hw=> //=.
+      move=> i he hw. by inversion hw.
+    move=> i h a he hw. case: v' he hw=> //= i' he hw. by inversion hw.
+  move=> es e t he hw. case: v' he hw=> //= i he hw. by inversion hw.
 (* var *)
 + move=> Gamma Sigma x t ht hteq bge vm m vm' m' v hv. inversion hv; subst.
   (* local *)
-  + by have := deref_addr_val_ty bge (vtype x) m' l ofs Full v H3.
+  + by have := wderef_addr_val_ty bge (vtype x) m' l ofs Full v H3.
   (* global *)
-  + by have := deref_addr_val_ty bge (vtype x) m' l ofs Full v H4.
+  + by have := wderef_addr_val_ty bge (vtype x) m' l ofs Full v H4.
 (* const int *)
 + move=> Gamma Sigma t sz s i a hteq bge vm m vm' m' v hv. by inversion hv; subst.
 (* const long *)
@@ -490,13 +618,14 @@ apply type_expr_indP => //=.
 (* app *)
 + move=> Gamma Sigma e es rt ef ef' ts ef'' hie hies bge vm m vm' m' v hv.
   inversion hv; subst. move: (hie bge vm m vm2 m2 (Vloc l Ptrofs.zero) H2)=> het.
-  move: (hies bge vm3 m3 vm4 m4 vs H7)=> hest. by inversion H4; subst.
+  move: (hies bge vm3 m3 vm4 m4 vs H7)=> hest. inversion H4; subst.
+  by have := type_to_wtype v (get_rt_fundef (Internal fd)) H16.
 (* ref *)
 + move=> Gamma Sigma e ef h bt a hi bge vm m vm' m' v hv. by inversion hv; subst.
 (* deref *)
 + move=> Gamma Sigma e ef h bt a hi bge vm m vm' m' v hv. inversion hv; subst.
   move: (hi bge vm m vm' m' (Vloc l ofs) H3)=> hlt. 
-  have hvt := deref_addr_val_ty bge (typeof_expr e) m l ofs bf v H7.
+  have hvt := wderef_addr_val_ty bge (typeof_expr e) m l ofs bf v H7.
   by rewrite H0 /= in hvt.
 (* massgn *)
 + move=> Gamma Sigma e1 e2 ef1 ef2 h bt a hi1 hi2 bge vm m vm' m' v hv.
@@ -554,18 +683,31 @@ Qed.
 Lemma subject_rreduction : forall m e v Gamma Sigma ef t, 
 bsem_expr_srv bge benv m e v ->
 type_expr Gamma Sigma e ef t ->
-typeof_value v (wtype_of_type t).
+wtypeof_value v (wtype_of_type t).
 Proof.
-move=> m e v Gamma Sigma ef t hr. move: Gamma Sigma ef t.
+move=> m e v Gamma Sigma ef t hr ht. move: Gamma Sigma ef t ht.
 induction hr=> //=. 
 (* Val *)
 + move=> Gamma Sigma ef t' ht. 
-  by inversion ht; subst; rewrite /typeof_value /wtype_of_type.
+  inversion ht; subst; rewrite /wtypeof_value /= /wtype_of_type.
+  case: t' ht H=> //=.  
+  + move=> p. case: p=> //=.
+    + case: v=> //=.
+      + move=> i ht hw. by inversion hw.
+      + move=> i ht hw. by inversion hw.
+      move=> l ofs ht hw. by inversion hw.
+    + move=> i s a ht hw. case: v ht hw=> //=.
+      + move=> l ht hw. by inversion hw.
+      move=> l ofs ht hw. by inversion hw. 
+    + move=> s a ht hw. case: v ht hw=> //=.
+      move=> l ht hw. by inversion hw.
+    move=> h b a. case: v=> //= i ht hw. by inversion hw. 
+  move=> h b a ht hw. case: v ht hw=> //= i ht hw. by inversion hw. 
 (* Deref *)
 + move=> Gamma Sigma ef t' ht.
   inversion ht; subst. rewrite H7.
   have := subject_lredcution hm e l ofs Gamma Sigma ef0 (Reftype h (Bprim bt) a) H H9=> hlt.
-  by have := deref_addr_val_ty bge (typeof_expr e) hm l.(lname) ofs l.(lbitfield) v H0.
+  by have := wderef_addr_val_ty bge (typeof_expr e) hm l.(lname) ofs l.(lbitfield) v H0.
 (* Uop *)
 + move=> Gamma Sigma ef t' ht. inversion ht; subst.
   move: (IHhr Gamma Sigma ef (typeof_expr e) H10)=> hvt.
@@ -580,28 +722,6 @@ induction hr=> //=.
   by have := cval_bval_type_eq v ct1 v' (typeof_expr e1) g g' i hvt H3 H; case: H1=> [] h1 h2; subst.
 Qed.
 
-(*Lemma subject_bstep_exprst : forall Gamma Sigma e ef t f k vm m e' k' vm' m',
-type_expr Gamma Sigma e ef t ->
-((Smallstep.plus bstep bge benv (ExprState f e k vm m) (ExprState f e' k' vm' m')) \/
-(Smallstep.star bstep bge benv (ExprState f e k vm m) (ExprState f e' k' vm' m'))) ->
-type_expr Gamma Sigma e' ef t.
-Proof.
-apply leftcontext_leftcontextlist_ind.
-move=> Gamma Sigma e ef t f k vm m e' k' vm' m' hte he.
-move: Gamma Sigma ef t f k vm m e' k' vm' m' he hte.
-elim: e=> //=.
-(* val *)
-+ move=> v t Gamma Sigma ef t' f k vm m e' k' vm' m' he hte.
-  inversion he; subst.
-  (* val *)
-  + by inversion H9.
-  (* deref *)
-  + 
-  inversion hte; subst. inversion he; subst.
-  (* .. *)
-  + by inversion H9.
-  + inversion H5*)
-
 End Subject_Reduction.
 
 (* Subject reduction : Small step semantics *)
@@ -613,8 +733,8 @@ type_expr Gamma Sigma e' ef t.
 Proof.
 move=> Gamma Sigma genv ef t vm e m e' m' ht he.
 induction he=> //=.
-+ inversion ht; subst. rewrite H0. by apply Ty_addr with h t0 a. 
-+ inversion ht; subst. rewrite H0. by apply Ty_addr with h t0 a.
++ inversion ht; subst. rewrite H0. by apply ty_addr with h t0 a. 
++ inversion ht; subst. rewrite H0. by apply ty_addr with h t0 a.
 Qed.
 
 
